ValidAccesses.v
@@ -12,76 +12,84 @@ Definition valid_accesses (m : mem) (t : tm) :=
 (* auxiliary                                                                 *)
 (* ------------------------------------------------------------------------- *)
 
-Lemma va_length : forall m t ad,
+Lemma vac_length : forall m t ad,
   valid_accesses m t ->
   access m t ad ->
-  ad < length m.
+  ad < #m.
 Proof.
-  intros * Hva Hacc. decompose sum (lt_eq_lt_dec ad (length m)); subst; trivial.
-  - specialize (Hva (length m) Hacc). lia.
-  - specialize (Hva ad Hacc). lia.
+  intros * Hvac Hacc.
+  decompose sum (lt_eq_lt_dec ad (#m)); subst; trivial.
+  - specialize (Hvac (#m) Hacc). lia.
+  - specialize (Hvac ad Hacc). lia.
 Qed.
 
-Lemma va_nacc_length : forall m t,
+Lemma vac_nacc_length : forall m t,
   valid_accesses m t ->
-  ~ access m t (length m).
+  ~ access m t (#m).
 Proof.
-  intros * ? F. eapply va_length in F; eauto. lia.
+  intros * ? F. eapply vac_length in F; eauto. lia.
 Qed.
 
 (* ------------------------------------------------------------------------- *)
-(* va constructors                                                           *)
+(* constructors                                                              *)
 (* ------------------------------------------------------------------------- *)
 
-Local Ltac solve_constructor_va := 
-  intros; intros ? ?; inversion_access; eauto.
+Local Ltac solve_vac_constructor := 
+  intros; intros ? ?; inversion_acc; eauto.
 
-Local Lemma va_new: forall m t T,
+Local Lemma vac_unit : forall m,
+  valid_accesses m <{ unit }>.
+Proof. solve_vac_constructor. Qed.
+
+Local Lemma vac_num : forall m n,
+  valid_accesses m <{ N n }>.
+Proof. solve_vac_constructor. Qed.
+
+Local Lemma vac_new : forall m t T,
   valid_accesses m t ->
   valid_accesses m <{ new T t }>.
-Proof. solve_constructor_va. Qed.
+Proof. solve_vac_constructor. Qed.
 
-Local Lemma va_load : forall m t,
+Local Lemma vac_load : forall m t,
   valid_accesses m t ->
   valid_accesses m <{ *t }>.
-Proof. solve_constructor_va. Qed.
+Proof. solve_vac_constructor. Qed.
 
-Local Lemma va_asg : forall m t1 t2,
+Local Lemma vac_asg : forall m t1 t2,
   valid_accesses m t1 ->
   valid_accesses m t2 ->
   valid_accesses m <{ t1 = t2 }>.
-Proof. solve_constructor_va. Qed.
+Proof. solve_vac_constructor. Qed.
 
-Local Lemma va_fun : forall m x Tx t,
+Local Lemma vac_var : forall m x,
+  valid_accesses m <{ var x }>.
+Proof. solve_vac_constructor. Qed.
+
+Local Lemma vac_fun : forall m x Tx t,
   valid_accesses m t ->
   valid_accesses m <{ fn x Tx --> t }>.
-Proof. solve_constructor_va. Qed.
+Proof. solve_vac_constructor. Qed.
 
-Local Lemma va_call : forall m t1 t2,
+Local Lemma vac_call : forall m t1 t2,
   valid_accesses m t1 ->
   valid_accesses m t2 ->
   valid_accesses m <{ call t1 t2 }>.
-Proof. solve_constructor_va. Qed.
+Proof. solve_vac_constructor. Qed.
 
-Local Lemma va_seq : forall m t1 t2,
+Local Lemma vac_seq : forall m t1 t2,
   valid_accesses m t1 ->
   valid_accesses m t2 ->
   valid_accesses m <{ t1; t2 }>.
-Proof. solve_constructor_va. Qed.
+Proof. solve_vac_constructor. Qed.
 
 (* ------------------------------------------------------------------------- *)
-(* inversion-va                                                              *)
+(* inversion                                                                 *)
 (* ------------------------------------------------------------------------- *)
 
-Local Ltac solve_inversion_va := 
-  intros; unfold valid_accesses in *;
-  match goal with
-  | [ |- _ /\ _ ] => split
-  | [ |- _ ] => idtac
-  end;
-  eauto using access.
+Local Ltac solve_vac_inversion := 
+  intros; unfold valid_accesses in *; try split; eauto using access.
 
-Local Lemma inversion_va_ref : forall m ad T,
+Local Lemma inv_vac_ref : forall m ad T,
   valid_accesses m <{ &ad :: T }> ->
   valid_accesses m m[ad].tm.
 Proof.
@@ -89,214 +97,234 @@ Proof.
   intros ad'. destruct (Nat.eq_dec ad ad'); subst; eauto using access.
 Qed.
 
-Local Lemma inversion_va_new : forall m t T,
+Local Lemma inv_vac_new : forall m t T,
   valid_accesses m <{ new T t }> ->
   valid_accesses m t.
-Proof. solve_inversion_va. Qed.
+Proof. solve_vac_inversion. Qed.
 
-Local Lemma inversion_va_load : forall m t,
+Local Lemma inv_vac_load : forall m t,
   valid_accesses m <{ *t }> ->
   valid_accesses m t.
-Proof. solve_inversion_va. Qed.
+Proof. solve_vac_inversion. Qed.
 
-Local Lemma inversion_va_asg : forall m t1 t2,
+Local Lemma inv_vac_asg : forall m t1 t2,
   valid_accesses m <{ t1 = t2 }> ->
   valid_accesses m t1 /\ valid_accesses m t2.
-Proof. solve_inversion_va. Qed.
+Proof. solve_vac_inversion. Qed.
 
-Local Lemma inversion_va_fun : forall m x Tx t,
+Local Lemma inv_vac_fun : forall m x Tx t,
   valid_accesses m <{ fn x Tx --> t }> ->
   valid_accesses m t.
-Proof. solve_inversion_va. Qed.
+Proof. solve_vac_inversion. Qed.
 
-Local Lemma inversion_va_call : forall m t1 t2,
+Local Lemma inv_vac_call : forall m t1 t2,
   valid_accesses m <{ call t1 t2 }> ->
   valid_accesses m t1 /\ valid_accesses m t2.
-Proof. solve_inversion_va. Qed.
+Proof. solve_vac_inversion. Qed.
 
-Local Lemma inversion_va_seq : forall m t1 t2,
+Local Lemma inv_vac_seq : forall m t1 t2,
   valid_accesses m <{ t1; t2 }> ->
   valid_accesses m t1 /\ valid_accesses m t2.
-Proof. solve_inversion_va. Qed.
+Proof. solve_vac_inversion. Qed.
 
-Ltac inversion_va :=
+Ltac inversion_vac :=
   match goal with
-    | [ H : valid_accesses _ <{ &_ :: _ }>      |- _ ] =>
-        eapply inversion_va_ref in H as Hwba'
-    | [ H : valid_accesses _ <{ new _ _ }>      |- _ ] =>
-        eapply inversion_va_new in H
-    | [ H : valid_accesses _ <{ *_ }>           |- _ ] =>
-        eapply inversion_va_load in H
-    | [ H : valid_accesses _ <{ _ = _ }>        |- _ ] => 
-        eapply inversion_va_asg in H as [? ?]
-    | [ H : valid_accesses _ <{ fn _ _ --> _ }> |- _ ] => 
-        eapply inversion_va_fun in H
-    | [ H : valid_accesses _ <{ call _ _ }>     |- _ ] => 
-        eapply inversion_va_call in H as [? ?]
-    | [ H : valid_accesses _ <{ _; _ }>         |- _ ] => 
-        eapply inversion_va_seq in H as [? ?]
+  | H: valid_accesses _ <{ &_ :: _  }> |- _ => eapply inv_vac_ref  in H as Hwba'
+  | H: valid_accesses _ <{ new _ _  }> |- _ => eapply inv_vac_new  in H
+  | H: valid_accesses _ <{ * _      }> |- _ => eapply inv_vac_load in H
+  | H: valid_accesses _ <{ _ = _    }> |- _ => eapply inv_vac_asg  in H as [? ?]
+  | H: valid_accesses _ <{ fn _ _ --> _ }> |- _ => eapply inv_vac_fun in H
+  | H: valid_accesses _ <{ call _ _ }> |- _ => eapply inv_vac_call in H as [? ?]
+  | H: valid_accesses _ <{ _ ; _    }> |- _ => eapply inv_vac_seq  in H as [? ?]
   end.
 
 (* ------------------------------------------------------------------------- *)
-(* va -- value, mem & subst                                                  *)
+(* preservation helpers                                                      *)
 (* ------------------------------------------------------------------------- *)
 
-Local Lemma va_alloc_value : forall m t t' ad v V,
+Local Lemma step_write_value_vac : forall m t t' ad v Tr,
   valid_accesses m t ->
-  t --[EF_Alloc ad v V]--> t' ->
+  t --[EF_Write ad v Tr]--> t' ->
   valid_accesses m v.
 Proof.
-  intros. induction_step; inversion_va; eauto using access.
+  intros. induction_step; inversion_vac; eauto using access.
 Qed.
 
-Local Lemma va_write_value : forall m t t' ad v V,
-  valid_accesses m t ->
-  t --[EF_Write ad v V]--> t' ->
-  valid_accesses m v.
-Proof.
-  intros. induction_step; inversion_va; eauto using access.
-Qed.
-
-Local Lemma va_added_value : forall m v V T,
-  valid_accesses (m +++ (v, V)) v ->
-  valid_accesses (m +++ (v, V)) <{ &(length m) :: T }>.
-Proof.
-  intros * ? ? Hacc.
-  remember (m +++ (v, V)) as m'.
-  remember (<{ &(length m) :: T }>) as t'.
-  induction Hacc; inversion Heqt'; subst.
-  - simpl_array. eauto using access.
-  - rewrite add_increments_length. lia.
-Qed.
-
-Local Lemma va_mem_add : forall m t v V,
-  valid_accesses m t ->
-  valid_accesses (m +++ (v, V)) t.
-Proof.
-  intros * Hva ? Hacc. induction Hacc; subst; inversion_va; eauto.
-  - eapply IHHacc. intros ? ?.
-    destruct (lt_eq_lt_dec ad' (length m)) as [[? | ?] | ?]; subst;
-    simpl_array; eauto; simpl in *; try solve [inversion_access].
-    specialize (Hva (length m) (access_ref m (length m) _)). lia.
-  - rewrite add_increments_length. eauto using access, Nat.lt_lt_succ_r.
-Qed.
-
-Local Lemma va_mem_set : forall m t ad v V,
-  valid_accesses m v ->
-  valid_accesses m t ->
-  valid_accesses m[ad <- (v, V)] t.
-Proof.
-  intros * ? ? ? Hacc.
-  rewrite set_preserves_length.
-  induction Hacc; inversion_va; eauto using access.
-  destruct (Nat.eq_dec ad ad'); subst;
-  assert (ad' < length m) by eauto using access;
-  simpl_array; eauto using access.
-Qed.
-
-Local Lemma va_subst : forall m t tx x,
+Local Lemma subst_vac : forall m t tx x,
   valid_accesses m t ->
   valid_accesses m tx ->
   valid_accesses m ([x := tx] t).
 Proof.
   intros. induction t;
-  try inversion_va; simpl; try (destruct String.string_dec);
-  eauto using va_new, va_load, va_asg, va_call, va_seq, va_fun.
-  intros ? F. inversion F.
+  try inversion_vac; simpl; try (destruct String.string_dec);
+  eauto using vac_new, vac_load, vac_asg, vac_call, vac_seq, vac_fun.
+  intros ? ?. inversion_acc.
+Qed.
+
+Local Lemma mem_add_vac : forall m t v Tr,
+  valid_accesses m t ->
+  valid_accesses (m +++ (v, Tr)) t.
+Proof.
+  intros * Hvac ? Hacc. induction Hacc; subst; inversion_vac; eauto.
+  - eapply IHHacc. intros ? ?.
+    destruct (lt_eq_lt_dec ad' (#m)) as [[? | ?] | ?]; subst;
+    simpl_array; eauto; simpl in *; try inversion_acc.
+    specialize (Hvac (#m) (acc_ref m (#m) _)). lia.
+  - rewrite add_increments_length. eauto using access, Nat.lt_lt_succ_r.
+Qed.
+
+Local Lemma mem_set_vac : forall m t ad v Tr,
+  valid_accesses m v ->
+  valid_accesses m t ->
+  valid_accesses m[ad <- (v, Tr)] t.
+Proof.
+  intros * ? ? ? Hacc. rewrite set_preserves_length.
+  induction Hacc; inversion_vac; eauto using access.
+  destruct (Nat.eq_dec ad ad'); subst;
+  assert (ad' < #m) by eauto using access;
+  simpl_array; eauto using access.
 Qed.
 
 (* ------------------------------------------------------------------------- *)
-(* valid-accesses-preservation                                               *)
+(* term preservation                                                         *)
 (* ------------------------------------------------------------------------- *)
 
-Local Lemma va_none_preservation : forall m t t',
+Local Lemma step_none_vac_preservation : forall m t t',
   valid_accesses m t ->
   t --[EF_None]--> t' ->
   valid_accesses m t'.
 Proof.
-  intros. induction_step; inversion_va;
-  eauto using va_new, va_load, va_asg, va_fun, va_call, va_seq. 
-  inversion_va. eauto using va_subst.
+  intros. induction_step; inversion_vac;
+  eauto using vac_new, vac_load, vac_asg, vac_fun, vac_call, vac_seq.
+  inversion_vac. eauto using subst_vac.
 Qed.
 
-Local Lemma va_alloc_preservation : forall m t t' v V,
+Local Lemma step_alloc_vac_preservation : forall m t t' v Tr,
   valid_accesses m t ->
-  t --[EF_Alloc (length m) v V]--> t' ->
-  valid_accesses (m +++ (v, V)) t'.
+  t --[EF_Alloc (#m) v Tr]--> t' ->
+  valid_accesses (m +++ (v, Tr)) t'.
 Proof.
-  intros. induction_step; inversion_va;
-  eauto using va_new, va_load, va_asg, va_call, va_seq, va_mem_add,
-    va_added_value. 
+  intros. induction_step; inversion_vac;
+  eauto using mem_add_vac, vac_new, vac_load, vac_asg, vac_call, vac_seq.
+  assert (valid_accesses (m +++ (v, Tr)) v) by eauto using mem_add_vac.
+  intros ? Hacc.
+  remember (m +++ (v, Tr)) as m'.
+  remember (<{ &(#m) :: Tr }>) as t'.
+  induction Hacc; inversion Heqt'; subst.
+  - simpl_array. eauto using access.
+  - rewrite add_increments_length. lia.
 Qed.
 
-Local Lemma va_read_preservation : forall m t t' ad,
+Local Lemma step_read_vac_preservation : forall m t t' ad,
   valid_accesses m t ->
   t --[EF_Read ad m[ad].tm]--> t' ->
   valid_accesses m t'.
 Proof.
-  intros. induction_step; inversion_va;
-  eauto using va_new, va_load, va_asg, va_call, va_seq.
+  intros. induction_step; inversion_vac;
+  eauto using vac_new, vac_load, vac_asg, vac_call, vac_seq.
   intros ad' ?. destruct (Nat.eq_dec ad ad'); subst; eauto using access.
 Qed.
 
-Local Lemma va_write_preservation : forall m t t' ad v V,
+Local Lemma step_write_vac_preservation : forall m t t' ad v Tr,
   valid_accesses m t ->
-  t --[EF_Write ad v V]--> t' ->
-  valid_accesses m[ad <- (v, V)] t'.
+  t --[EF_Write ad v Tr]--> t' ->
+  valid_accesses m[ad <- (v, Tr)] t'.
 Proof.
-  intros. assert (valid_accesses m v); eauto using va_write_value.
-  induction_step; inversion_va;
-  eauto using va_new, va_load, va_asg, va_call, va_seq, va_mem_set.
-  intros ? ?. inversion_access.
+  intros. assert (valid_accesses m v) by eauto using step_write_value_vac.
+  induction_step; inversion_vac;
+  eauto using mem_set_vac, vac_unit, vac_new, vac_load, vac_asg,
+    vac_call, vac_seq.
 Qed.
 
-Theorem va_mstep_preservation : forall m m' t t' eff,
+Local Corollary mstep_vac_preservation : forall m m' t t' eff,
   valid_accesses m t ->
   m / t ==[eff]==> m' / t' ->
   valid_accesses m' t'.
 Proof.
   intros. inversion_mstep;
-  eauto using va_none_preservation,
-    va_alloc_preservation,
-    va_read_preservation,
-    va_write_preservation.
+  eauto using step_none_vac_preservation,
+    step_alloc_vac_preservation,
+    step_read_vac_preservation,
+    step_write_vac_preservation.
+Qed.
+
+Local Lemma step_spawn_vac_preservation : forall m t t' block,
+  valid_accesses m t ->
+  t --[EF_Spawn block]--> t' ->
+  valid_accesses m t'.
+Proof.
+  intros. induction_step; try inversion_vac;
+  eauto using vac_unit, vac_new, vac_load, vac_asg, vac_call, vac_seq.
 Qed.
 
 (* ------------------------------------------------------------------------- *)
-(* memory valid-accesses preservation                                        *)
+(* memory preservation                                                       *)
 (* ------------------------------------------------------------------------- *)
 
-Local Lemma mva_alloc_preservation : forall m t t' v V,
+Local Lemma step_alloc_mem_vac_preservation : forall m t t' v Tr,
   valid_accesses m t ->
   forall_memory m (valid_accesses m) ->
-  t --[EF_Alloc (length m) v V]--> t' ->
-  forall_memory (m +++ (v, V)) (valid_accesses (m +++ (v, V))).
+  t --[EF_Alloc (#m) v Tr]--> t' ->
+  forall_memory (m +++ (v, Tr)) (valid_accesses (m +++ (v, Tr))).
 Proof.
-  intros * Hva ? ? ad. induction_step; inversion_va; eauto.
-  decompose sum (lt_eq_lt_dec ad (length m)); subst;
-  simpl_array; eauto using va_mem_add.
-  intros ? ?. simpl in *. inversion_access.
+  intros * Hvac ? ? ad. induction_step; inversion_vac; eauto;
+  decompose sum (lt_eq_lt_dec ad (#m)); subst;
+  simpl_array; eauto using mem_add_vac.
+  unfold memory_default. simpl. eauto using vac_unit.
 Qed.
 
-Local Lemma mva_write_preservation : forall m t t' ad v V,
+Local Lemma step_write_mem_vac_preservation : forall m t t' ad v Tr,
   valid_accesses m t ->
   forall_memory m (valid_accesses m) ->
-  t --[EF_Write ad v V]--> t' ->
-  forall_memory m[ad <- (v, V)] (valid_accesses m[ad <- (v, V)]).
+  t --[EF_Write ad v Tr]--> t' ->
+  forall_memory m[ad <- (v, Tr)] (valid_accesses m[ad <- (v, Tr)]).
 Proof.
-  intros * Hva Hmva ? ad'. induction_step; inversion_va; eauto.
+  intros * Hvac Hmvac ? ad'. induction_step; inversion_vac; eauto.
   decompose sum (lt_eq_lt_dec ad ad'); subst;
-  try (assert (ad' < length m) by eauto using access);
-  simpl_array; eauto using va_mem_set.
+  try (assert (ad' < #m) by eauto using access);
+  simpl_array; eauto using mem_set_vac.
 Qed.
 
-Theorem mva_mstep_preservation : forall m m' t t' eff,
+Local Corollary mstep_mem_vac_preservation : forall m m' t t' eff,
   valid_accesses m t ->
   forall_memory m (valid_accesses m) ->
   m / t ==[eff]==> m' / t' ->
   forall_memory m' (valid_accesses m').
 Proof.
   intros. inversion_mstep;
-  eauto using mva_alloc_preservation, mva_write_preservation.
+  eauto using step_alloc_mem_vac_preservation, step_write_mem_vac_preservation.
+Qed.
+
+(* ------------------------------------------------------------------------- *)
+(* preservation                                                              *)
+(* ------------------------------------------------------------------------- *)
+
+Local Lemma step_spawn_block_vac : forall m t t' block,
+  t --[EF_Spawn block]--> t' ->
+  valid_accesses m block.
+Proof.
+Abort.
+
+Theorem valid_accesses_term_preservation : forall m m' ths ths' tid eff,
+  forall_memory m (valid_accesses m) ->
+  forall_threads ths (valid_accesses m) ->
+  m / ths ~~[tid, eff]~~> m' / ths' ->
+  forall_threads ths' (valid_accesses m').
+Proof.
+  intros. eapply cstep_preservation; eauto; intros.
+  - eauto using mstep_vac_preservation.
+  - inversion_mstep; eauto using mem_add_vac, mem_set_vac, step_write_value_vac.
+  - admit.
+  - eauto using step_spawn_vac_preservation.
+  - unfold thread_default. eauto using vac_unit.
+Abort.
+
+Theorem valid_accesses_memory_preservation : forall m m' ths ths' tid eff,
+  forall_threads ths (valid_accesses m) ->
+  forall_memory m (valid_accesses m) ->
+  m / ths ~~[tid, eff]~~> m' / ths' ->
+  forall_memory m' (valid_accesses m').
+Proof.
+  intros. inversion_cstep; eauto using mstep_mem_vac_preservation.
 Qed.
 
